import Relation.Binary.PropositionalEquality as Eq
open Eq using (_â‰¡_; refl; cong; congâ‚‚)

data Type : Set where
  ðŸ˜ ðŸ™ âŠ¥ âŠ¤ : Type
  Â¡ Â¿ : Type -> Type
  _&_ _âŠ•_ _âŠ—_ _â…‹_ : Type -> Type -> Type

data Dual : Type -> Type -> Set where
  d-ðŸ˜-âŠ¤ : Dual ðŸ˜ âŠ¤
  d-âŠ¤-ðŸ˜ : Dual âŠ¤ ðŸ˜
  d-ðŸ™-âŠ¥ : Dual ðŸ™ âŠ¥
  d-âŠ¥-ðŸ™ : Dual âŠ¥ ðŸ™
  d-!-? : âˆ€{A B} -> Dual A B -> Dual (Â¡ A) (Â¿ B)
  d-?-! : âˆ€{A B} -> Dual A B -> Dual (Â¿ A) (Â¡ B)
  d-&-âŠ• : âˆ€{A B A' B'} -> Dual A A' -> Dual B B' -> Dual (A & B) (A' âŠ• B')
  d-âŠ•-& : âˆ€{A B A' B'} -> Dual A A' -> Dual B B' -> Dual (A âŠ• B) (A' & B')
  d-âŠ—-â…‹ : âˆ€{A B A' B'} -> Dual A A' -> Dual B B' -> Dual (A âŠ— B) (A' â…‹ B')
  d-â…‹-âŠ— : âˆ€{A B A' B'} -> Dual A A' -> Dual B B' -> Dual (A â…‹ B) (A' âŠ— B')

dual-symm : âˆ€{A B} -> Dual A B -> Dual B A
dual-symm d-ðŸ˜-âŠ¤ = d-âŠ¤-ðŸ˜
dual-symm d-âŠ¤-ðŸ˜ = d-ðŸ˜-âŠ¤
dual-symm d-ðŸ™-âŠ¥ = d-âŠ¥-ðŸ™
dual-symm d-âŠ¥-ðŸ™ = d-ðŸ™-âŠ¥
dual-symm (d-!-? p) = d-?-! (dual-symm p)
dual-symm (d-?-! p) = d-!-? (dual-symm p)
dual-symm (d-&-âŠ• p q) = d-âŠ•-& (dual-symm p) (dual-symm q)
dual-symm (d-âŠ•-& p q) = d-&-âŠ• (dual-symm p) (dual-symm q)
dual-symm (d-âŠ—-â…‹ p q) = d-â…‹-âŠ— (dual-symm p) (dual-symm q)
dual-symm (d-â…‹-âŠ— p q) = d-âŠ—-â…‹ (dual-symm p) (dual-symm q)

dual-inv : âˆ€{A B C} -> Dual A B -> Dual B C -> A â‰¡ C
dual-inv d-ðŸ˜-âŠ¤ d-âŠ¤-ðŸ˜ = refl
dual-inv d-âŠ¤-ðŸ˜ d-ðŸ˜-âŠ¤ = refl
dual-inv d-ðŸ™-âŠ¥ d-âŠ¥-ðŸ™ = refl
dual-inv d-âŠ¥-ðŸ™ d-ðŸ™-âŠ¥ = refl
dual-inv (d-!-? p) (d-?-! q) = cong Â¡ (dual-inv p q)
dual-inv (d-?-! p) (d-!-? q) = cong Â¿ (dual-inv p q)
dual-inv (d-&-âŠ• p q) (d-âŠ•-& r s) = congâ‚‚ _&_ (dual-inv p r) (dual-inv q s)
dual-inv (d-âŠ•-& p q) (d-&-âŠ• r s) = congâ‚‚ _âŠ•_ (dual-inv p r) (dual-inv q s)
dual-inv (d-âŠ—-â…‹ p q) (d-â…‹-âŠ— r s) = congâ‚‚ _âŠ—_ (dual-inv p r) (dual-inv q s)
dual-inv (d-â…‹-âŠ— p q) (d-âŠ—-â…‹ r s) = congâ‚‚ _â…‹_ (dual-inv p r) (dual-inv q s)

dual-fun-r : âˆ€{A B C} -> Dual A B -> Dual A C -> B â‰¡ C
dual-fun-r d e = dual-inv (dual-symm d) e

dual-fun-l : âˆ€{A B C} -> Dual B A -> Dual C A -> B â‰¡ C
dual-fun-l d e = dual-inv d (dual-symm e)
